\documentclass{unswmaths}
\usepackage{color}
\usepackage{unswshortcuts}
\begin{document}
\author{Adam J. Gray}
\studentno{3329798}
\subject{Number Theory}
\title{Assignment}

\unswtitle

\section{Question 4}

\begin{align*}
	I_n &= \sum_{j=0}^{n-1} \Delta_j (M_{j+1} - M_j) & n = 1,\ldots, N \\
\end{align*}

See that

\begin{align*}
	\E{I_{n+1} | F_n } &= \E{\sum_{j=0}^{n} \Delta_j (M_{j+1} - M_j) | \mathcal{F}_n} \\
		&= \E{\sum_{j=0}^{n-1} \Delta_j (M_{j+1} - M_j) + \Delta_n(M_{n+1} - M_{n}) | \mathcal{F}_n} \\
		&= \E{\sum_{j=0}^{n-1} \Delta_j (M_{j+1} - M_j) | \mathcal{F}_n} + \E{\Delta_n(M_{n+1} - M_{n}) | \mathcal{F}_n} \\
		& \text{ by linearity of conditional expectation } \\
		&= I_n + \Delta_n \E{M_{n+1} - \E{M_n} | \mathcal{F}} \\
		& \text{ because } \Delta_n \text{ is adapted to } \mathcal{F}_n \\
		&= I_n + \Delta_n (\E{M_{n+1} | \mathcal{F}} - M_n) \\
		& \text{ because } M_n \text{ is completely determined by } \mathcal{F}_n \\
		&= I_n + \Delta_n (M_n - M_n) \\
		& \text{ because } M_n \text{ is a martingale } \\
		&= I_n
\end{align*}

and so $ \{ I_n \}_{n=0}^{N} $ is a martingale.
\end{document}


